rewriting_system.v
@@ -2,18 +2,17 @@ Require Import Relations.
 
 
 
-Class REWRITING_SYSTEM :=
+Class REWRITING_SYSTEM (configuration : Set) :=
 {
-    configuration : Set;
-    transition    : configuration -> configuration -> Prop
+    transition : configuration -> configuration -> Prop
 }.
 
 
-Notation "`( rw ) c1 → c2"  := (@transition rw c1 c2)
+Notation "`( rw ) c1 → c2"  := (@transition _ rw c1 c2)
                                          (no associativity, at level 70, c1 at level 69).
-Notation "`( rw ) c1 →+ c2" := (clos_trans_1n _ (@transition rw) c1 c2)
+Notation "`( rw ) c1 →+ c2" := (clos_trans_1n _ (@transition _ rw) c1 c2)
                                          (no associativity, at level 70, c1 at level 69).
-Notation "`( rw ) c1 →* c2" := (clos_refl_trans_1n _ (@transition rw) c1 c2)
+Notation "`( rw ) c1 →* c2" := (clos_refl_trans_1n _ (@transition _ rw) c1 c2)
                                          (no associativity, at level 70, c1 at level 69).
 
 Notation "c1 → c2"  := (transition c1 c2)                (no associativity, at level 70).
@@ -24,20 +23,17 @@ Notation "c1 →* c2" := (clos_refl_trans_1n _ transition c1 c2)
 
 
 
-
-Class LABELED_REWRITING_SYSTEM :=
+Class LABELED_REWRITING_SYSTEM (label lconfiguration : Set) :=
 {
-    label          : Set; 
-    lconfiguration : Set;
-    ltransition    : label -> lconfiguration -> lconfiguration -> Prop
+    ltransition : label -> lconfiguration -> lconfiguration -> Prop
 }.
 
 
-Notation "`( rw ) l |~ c1 → c2"  := (@ltransition rw l c1 c2)
+Notation "`( rw ) l |~ c1 → c2"  := (@ltransition _ _ rw l c1 c2)
                                       (no associativity, at level 70, c1, l at level 69).
-Notation "`( rw ) l |~ c1 →+ c2" := (clos_trans_1n _ (@ltransition rw l) c1 c2)
+Notation "`( rw ) l |~ c1 →+ c2" := (clos_trans_1n _ (@ltransition _ _ rw l) c1 c2)
                                       (no associativity, at level 70, c1, l at level 69).
-Notation "`( rw ) l |~ c1 →* c2" := (clos_refl_trans_1n _ (@ltransition rw l) c1 c2)
+Notation "`( rw ) l |~ c1 →* c2" := (clos_refl_trans_1n _ (@ltransition _ _ rw l) c1 c2)
                                       (no associativity, at level 70, c1, l at level 69).
 
 Notation "l |~ c1 → c2"  := (ltransition l c1 c2)
@@ -49,9 +45,7 @@ Notation "l |~ c1 →* c2" := (clos_refl_trans_1n _ (ltransition l) c1 c2)
 
 
 
-Instance LRWS_is_RWS (_ : REWRITING_SYSTEM) : LABELED_REWRITING_SYSTEM :=
+Instance LRWS_is_RWS {conf} `(REWRITING_SYSTEM conf) : LABELED_REWRITING_SYSTEM unit conf:=
 {
-    label          := unit;
-    lconfiguration := configuration;
-    ltransition    := fun (_ : unit) => transition
+    ltransition := fun (_ : unit) => transition
 }.
