rewriting_system_following.v
@@ -12,9 +12,11 @@ end.
 Coercion fin_lift1 : Fin.t >-> Fin.t.
 
 
-Class RW_FOLLOWING (Follower Followed : REWRITING_SYSTEM) :=
+Class RW_FOLLOWING                                    {configuration_er configuration_ed}
+    (Follower : REWRITING_SYSTEM configuration_er) 
+    (Followed : REWRITING_SYSTEM configuration_ed) :=
 {
-    semantics : (@configuration Follower) -> (@configuration Followed);
+    semantics : configuration_er -> configuration_ed;
 
     correct :                                                             forall cr1 cr2,
         `(Follower) cr1 → cr2  ->  semantics cr1 = semantics cr2  \/  
@@ -22,14 +24,14 @@ Class RW_FOLLOWING (Follower Followed : REWRITING_SYSTEM) :=
 
     complete :                                                        forall cd1 cd2 cr1,
         `(Followed) cd1 → cd2  ->  semantics cr1 = cd1 -> 
-            exists n (crs : Vector.t configuration n) cr2,
+            exists n (crs : Vector.t configuration_er n) cr2,
             (**)Forall (fun cr => semantics cr = cd1) crs /\
             (**)semantics cr2 = cd2                       /\
             (**)forall m : Fin.t (n+1), 
                     (cr1 :: crs ++ [cr2])[@m] → (crs ++ [cr2])[@m];
 
     no_silent_loops :
-      ~ exists crs : nat -> configuration, (*a stream of configurations*)
+      ~ exists crs : nat -> configuration_er, (*a stream of configurations*)
           forall n, 
           (**)  `(Follower) crs n  →  crs (S n)  /\ 
           (**)~ `(Followed) semantics (crs n)  →  semantics (crs (S n))
