Entropy.v
@@ -4,4 +4,6 @@ Parameters
 (entropy  : Set)
 (draw_fin : entropy -> forall n, Fin.t n).
 
-Axiom draw_fin_correct : forall n m, exists e, draw_fin e n = m.
+Axioms
+(draw_fin_correct : forall n m, exists e, draw_fin e n = m)
+(entropy_exists   : exists (_ : entropy), True).
