Subset.v
@@ -1,0 +1,100 @@
+
+Class CompPred U (P : U -> Prop) :=
+{ satisfyingness_comp : forall x, {P x} + {~P x} }.
+
+
+Definition is_satisfied {U} P `{CompPred U P} x := satisfyingness_comp x.
+
+
+Definition satisfied {U} P `{CompPred U P} x : Prop :=
+    if is_satisfied P x then True else False.
+
+
+Definition subset {U} P `{CompPred U P} := { x : U | satisfied P x }.
+
+Notation "x ? P " := (satisfied P x) (no associativity, at level 89).
+Notation "{? U | P }" := (@subset U P _) (U at level 0).
+Notation "¹ x" := (proj1_sig x) (at level 0).
+(* Bad without eta_CompPred :
+Notation "{ x : U |? P }" := (@subset U (fun x => P) _). *)
+
+
+
+Definition sat_token                                          {U} P `{CompPred U P} {x} :
+    P x -> x ? P :=
+
+    fun H0 => match is_satisfied P x as s
+              return (if s then True else False) : Prop
+              with
+              | left _ => I
+              | right notH0 => notH0 H0 
+              end.
+
+Definition sat_untoken                                          {U} P `{CompPred U P} x :
+    x ? P -> P x :=
+
+    fun W  => match is_satisfied P x as s 
+              return ((if s then True else False) : Prop) -> _ 
+              with
+              | left H      => fun _ => H
+              | right notH0 => fun devil => match devil with end
+              end W.
+
+Notation "H '`as' 'witness' 'of' P" := (sat_token P H) (no associativity, at level 73).
+Notation "W '`as' 'proof' 'of' P"   := (sat_untoken P W) (no associativity, at level 73).
+
+
+
+Instance not_CompPred                                                             {U} P :
+    CompPred U P -> CompPred U (fun x => ~P x) :=
+
+{
+    satisfyingness_comp := fun x =>
+        match is_satisfied P x with
+        | left H  => right (fun notH => notH H)
+        | right H => left H
+        end
+}.
+
+
+Instance const_CompPred                                                          {U1} P :
+    CompPred U1 P -> forall U2 x,  CompPred U2 (fun _ => P x) :=
+
+{
+    satisfyingness_comp := fun _ => is_satisfied P x
+}. 
+
+
+Lemma sat_token_unique :                                  forall {U} P `{CompPred U P} x,
+      forall H1 H2 : x ? P, H1 = H2.
+
+Proof.
+  intros U P H x H1 H2.
+  unfold satisfied in *.
+  destruct (is_satisfied P x);
+  solve [destruct H1, H2; auto].
+Qed.
+
+
+Hint Resolve sat_token sat_token_unique.
+
+
+(*
+Instance eta_CompPred {U} P {H : CompPred U P} : CompPred U (fun x => P x) := H.
+*)
+
+(*
+Instance strange_CompPred {U} P {H : CompPred U P} : CompPred U P := H.
+*)
+
+(*
+Definition P (x : unit) := True.
+
+
+Instance udp : CompPred unit P. 
+  split; unfold P; auto. Defined.
+
+
+Definition S1 := subset (fun (x : unit) => P x).
+Definition S2 := subset (fun (x : unit) => ~True).
+*)
